procedures/recursivity/examples

Hoare.thy
@@ -1,82 +1,138 @@
 theory Hoare
-  imports While "$AFP/KAT_and_DRA/SingleSorted/KAT_Models"
+  imports While "$AFP/KAT_and_DRA/SingleSorted/KAT_Models" "$ISABELLE_HOME/src/HOL/Eisbach/Eisbach"
 begin
 
 no_notation comp_op ("n_" [90] 91)
   and test_operator  ("t_" [100] 101)
   and floor ("\<lfloor>_\<rfloor>")
   and ceiling ("\<lceil>_\<rceil>")
+  and Set.image (infixr "`" 90)
   
 notation inf (infixl "\<sqinter>" 60)
 
-definition ht :: "('v \<Rightarrow> 's set) \<Rightarrow> 's rel \<Rightarrow> ('v \<Rightarrow> 's set) \<Rightarrow> bool" where
-  "ht P x Q \<equiv> \<forall>u. \<lfloor>P u\<rfloor>;x \<subseteq> x;\<lfloor>Q u\<rfloor>"
+named_theorems hl_rules
 
-lemma hl_abort: "ht P abort Q"
+method hoare_step uses simp declares hl_rules = (
+  ((rule allI | rule ballI | subst simp)+)?;
+  (assumption | rule subset_refl | rule hl_rules)
+)
+
+method hoare uses simp declares hl_rules = 
+  (hoare_step; hoare?)+
+
+method hoarerule uses first simp declares hl_rules = 
+  (((rule allI | rule ballI | subst simp)+)?, rule first; hoare?)
+
+definition ht :: "'s set \<Rightarrow> 's rel \<Rightarrow> 's set \<Rightarrow> bool" where
+  "ht P x Q \<equiv> \<lfloor>P\<rfloor>;x \<subseteq> x;\<lfloor>Q\<rfloor>"
+
+lemma hl_abort [hl_rules]: "ht P abort Q"
   by (auto simp: ht_def abort_def seq_def)
   
-lemma hl_skip: "P \<le> Q \<Longrightarrow> ht P skip Q"
-  by (auto simp: ht_def skip_def le_fun_def seq_def)
+lemma hl_skip [hl_rules]: "P \<subseteq> Q \<Longrightarrow> ht P skip Q"
+  by (auto simp: ht_def skip_def seq_def)
   
-lemma hl_to_rel: "\<forall>u. P u \<subseteq> {s. f s \<in> Q u} \<Longrightarrow> ht P (\<langle>f\<rangle>) Q"
+lemma hl_to_rel [hl_rules]: "P \<subseteq> {s. f s \<in> Q} \<Longrightarrow> ht P (\<langle>f\<rangle>) Q"
   by (auto simp: ht_def to_rel_def seq_def)
 
-lemma hl_seq: "ht R y Q \<Longrightarrow> ht P x R \<Longrightarrow> ht P (x; y) Q"
+lemma hl_seq [hl_rules]: "ht R y Q \<Longrightarrow> ht P x R \<Longrightarrow> ht P (x; y) Q"
   by (force simp: ht_def seq_def)
 
-lemma hl_cond: "ht (<b> \<sqinter> P) x Q \<Longrightarrow> ht (-<b> \<sqinter> P) y Q \<Longrightarrow> ht P (cond b x y) Q"
-  by (fastforce simp: ht_def cond_def seq_def assert_def)
+lemma hl_split: "ht P x {t. Q t} \<Longrightarrow> ht P x {t. Q' t} \<Longrightarrow> ht P x {t. Q t \<and> Q' t}"
+  by (force simp: ht_def seq_def)
+
+lemma hl_cond : "ht (b \<sqinter> P) x Q \<Longrightarrow> ht (-b \<sqinter> P) y Q \<Longrightarrow> ht P (cond b x y) Q"
+  by (fastforce simp: ht_def cond_def seq_def)
+
+lemma hl_cond_tac [hl_rules]: "P \<subseteq> P' \<union> - b \<Longrightarrow> P \<subseteq> P''  \<union> b  \<Longrightarrow> ht P' x Q \<Longrightarrow> ht P'' y Q \<Longrightarrow> ht P (cond b x y) Q"
+  by (fastforce simp: ht_def cond_def seq_def)
   
-lemma hl_while: "ht (<b> \<sqinter> i) x i \<Longrightarrow> ht i (while b x) (-<b> \<sqinter> i)"
-proof (simp add: ht_def while_def seq_def, rule allI)
-  fix u
-  assume "\<forall>u. \<lfloor><b> u \<sqinter> i u\<rfloor> O x \<subseteq> x O \<lfloor>i u\<rfloor>"
-  hence "\<lfloor>i u\<rfloor> O (\<lfloor><b> u\<rfloor> O x)\<^sup>* \<subseteq> (\<lfloor><b> u\<rfloor> O x)\<^sup>* O \<lfloor>i u\<rfloor>"
+lemma hl_while: "ht (b \<sqinter> i) x i \<Longrightarrow> ht i (while b x) (-b \<sqinter> i)"
+proof (simp add: ht_def while_def seq_def)
+  assume "\<lfloor>b \<sqinter> i\<rfloor> O x \<subseteq> x O \<lfloor>i\<rfloor>"
+  hence "\<lfloor>i\<rfloor> O (\<lfloor>b\<rfloor> O x)\<^sup>* \<subseteq> (\<lfloor>b\<rfloor> O x)\<^sup>* O \<lfloor>i\<rfloor>"
     by (force intro!: rel_kat.star_sim2)
-  thus "\<lfloor>i u\<rfloor> O (\<lfloor>b\<rfloor> O x)\<^sup>* O \<lfloor>-b\<rfloor> \<subseteq> ((\<lfloor>b\<rfloor> O x)\<^sup>* O \<lfloor>-b\<rfloor>) O \<lfloor>-<b> u \<sqinter> i u\<rfloor>"
-    by (auto simp: assert_def)
+  thus "\<lfloor>i\<rfloor> O (\<lfloor>b\<rfloor> O x)\<^sup>* O \<lfloor>-b\<rfloor> \<subseteq> ((\<lfloor>b\<rfloor> O x)\<^sup>* O \<lfloor>-b\<rfloor>) O \<lfloor>-b \<sqinter> i\<rfloor>"
+    by auto
 qed
 
-lemma hl_dyn: "\<forall>u. \<forall>s \<in> P u. ht P (g s) Q \<Longrightarrow> ht P (\<lceil>g\<rceil>) Q"
+lemma hl_dyn [hl_rules]: "\<forall>s \<in> P. ht P (g s) Q \<Longrightarrow> ht P (\<lceil>g\<rceil>) Q"
   by (fastforce simp: ht_def seq_def dyn_def)
-  
+
 lemma hl_pre: "P \<le> P' \<Longrightarrow> ht P' x Q \<Longrightarrow> ht P x Q"
   by (fastforce simp: ht_def le_fun_def seq_def)
 
 lemma hl_post: "Q' \<le> Q \<Longrightarrow> ht P x Q' \<Longrightarrow> ht P x Q"
   by (fastforce simp: ht_def le_fun_def seq_def)
-  
-lemma hl_conseq: "ht P' x Q' \<Longrightarrow> P \<le> P' \<Longrightarrow> Q' \<le> Q \<Longrightarrow> ht P x Q"
-  by (metis hl_pre hl_post)
 
-lemma hl_block: "\<forall>u. P u \<subseteq> {s. init s \<in> P' s u} \<Longrightarrow> \<forall>s. ht (P' s) x (\<lambda>u. {t. ret s t \<in> R s t u}) 
+lemma hl_classic: "P \<le> P' \<Longrightarrow> Q' \<le> Q \<Longrightarrow> ht P' x Q' \<Longrightarrow> ht P x Q"
+  by (fastforce simp: ht_def le_fun_def seq_def)
+  
+lemma hl_conseq: "\<forall>s. ht (P' s) c (Q' s) \<Longrightarrow> \<forall>s. s \<in> P \<longrightarrow> (\<exists>s'. s \<in> P' s' \<and> (Q' s' \<subseteq> Q)) \<Longrightarrow> ht P c Q"
+  by (force simp: ht_def seq_def)
+
+lemma hl_block [hl_rules]: "P \<subseteq> {s. init s \<in> P' s} \<Longrightarrow> \<forall>s. ht (P' s) x {t. ret s t \<in> R s t}
   \<Longrightarrow> \<forall>s t. ht (R s t) (c s t) Q \<Longrightarrow> ht P (block init x ret c) Q"
-  apply (simp add: block_def)
-  apply (rule hl_dyn)
-  apply clarsimp
-  apply (rule hl_seq)
-  apply (rule hl_seq)
-  prefer 2
-  apply (erule_tac x=s in allE)
-  apply assumption
-  apply (rule hl_dyn)
-  apply clarsimp
-  apply (clarsimp simp: ht_def to_rel_def seq_def)
+  apply (rule hl_conseq [where P'="\<lambda>s'. {s. s = s' \<and> init s \<in> P' s'}" and Q'="\<lambda> s'. Q"])
+  apply (hoare_step simp: block_def, hoare_step)
+  apply (rule_tac R="{t. ret s t \<in> R s t}" in hl_seq)
+  apply (rule_tac P'="\<lambda>s'. {t. t=s' \<and> ret s t \<in> R s t}" and Q'="\<lambda>s'. Q" in hl_conseq)
+  apply hoare
+  apply (erule_tac x=sa in allE, erule_tac x=sc in allE, assumption)
+  apply force
+  apply force
+  apply (erule_tac x=s in allE, assumption)
+  apply hoare_step
+  apply force+
+ done
+
+lemma ht_true [intro]: "ht UNIV x UNIV"
+  by (auto simp: ht_def seq_def)
+
+lemma hl_false [intro]: "ht {} x {}"
+  by (auto simp: ht_def seq_def)
+
+lemma hl_Sup: "\<forall>x \<in> X. ht P x Q \<Longrightarrow> ht P (Sup X) Q"
+  by (fastforce simp: ht_def seq_def)
+thm allE
+lemma hl_rec [hl_rules]: "mono f \<Longrightarrow> (\<And>x. \<forall>z. ht (P z) x (Q z) \<Longrightarrow> \<forall>z. ht (P z) (f x) (Q z)) \<Longrightarrow> \<forall>z. ht (P z) (lfp f) (Q z)"
+
+  apply (rule lfp_ordinal_induct)
+apply simp
+apply force
+apply (auto intro: hl_Sup)
+done
+
+lemma hl_rec2 [hl_rules]: "mono f \<Longrightarrow> (\<And>x. \<forall>z. ht (P z) x (Q z) \<Longrightarrow> \<forall>z. ht (P z) (f z x) (Q z)) \<Longrightarrow> \<forall>z. ht (P z) (lfp (f z)) (Q z)"
 sorry
 
 text {* Annotated programs *}
 
-lemma hl_awhile: "P \<le> i \<Longrightarrow> -<b> \<sqinter> i \<le> Q \<Longrightarrow> ht (<b> \<sqinter> i) x i \<Longrightarrow> ht P (awhile i b x) Q"
-  by (auto simp: awhile_def intro: hl_while hl_conseq)
+lemma hl_awhile [hl_rules]: "P \<subseteq> i \<Longrightarrow> -b \<inter> i \<subseteq> Q \<Longrightarrow> ht (b \<sqinter> i) x i \<Longrightarrow> ht P (awhile i b x) Q"
+  by (hoarerule simp: awhile_def first: hl_conseq hl_rules: hl_while) force
+  
+lemma hl_apre: "P \<subseteq> P' \<Longrightarrow> ht P' x Q \<Longrightarrow> ht P (apre P' x) Q"
+  by (hoarerule simp: apre_def first: hl_pre)
 
-lemma hl_apre: "P \<le> P' \<Longrightarrow> ht P' x Q \<Longrightarrow> ht P (apre P' x) Q"
-  by (auto simp: apre_def intro: hl_pre)
+lemma hl_apre2: "\<forall>z. ht (P' z) x (Q' z) \<Longrightarrow> \<forall>s t. (\<forall>z. s \<in> P' z \<longrightarrow> t \<in> Q' z) \<longrightarrow> (\<forall>z. s \<in> P z \<longrightarrow> t \<in> Q z) \<Longrightarrow> \<forall>z. ht (P z) x (Q z)"
+  apply (simp add: apre_def seq_def ht_def)
+  apply auto
+  by force
+
+lemma hl_apre3: "\<forall>z. ht (P' z) x (Q' z) \<Longrightarrow> \<forall>s t. (\<forall>z. s \<in> P' z \<longrightarrow> t \<in> Q' z) \<longrightarrow> (\<forall>z. s \<in> P z \<longrightarrow> t \<in> Q z) \<Longrightarrow> ht (P z) x (Q z)"
+  apply (simp add: apre_def seq_def ht_def)
+  apply auto
+  by force
+
+lemma hl_2: "P \<subseteq> {s. (\<exists>z. s \<in> P' z \<and> Q' z \<subseteq> Q)} \<Longrightarrow> \<forall>z. ht (P' z) x (Q' z) 
+  \<Longrightarrow> ht P x Q"
+sorry
   
-lemma hl_apost: "Q' \<le> Q \<Longrightarrow> ht P x Q' \<Longrightarrow> ht P (apost x Q') Q"
-  by (auto simp: apost_def intro!: hl_seq hl_apre hl_skip)
+lemma hl_apost [hl_rules]: "Q' \<le> Q \<Longrightarrow> ht P x Q' \<Longrightarrow> ht P (apost x Q') Q"
+  by (auto simp: apost_def le_fun_def intro!: hl_seq hl_apre hl_skip)
   
-lemma hl_aprog: "P \<le> P' \<Longrightarrow> Q' \<le> Q \<Longrightarrow> ht P' x Q' \<Longrightarrow> ht P (aprog P' x Q') Q"
-  by (auto simp: aprog_def intro: hl_conseq)
+lemma hl_aprog [hl_rules]: "P \<le> P' \<Longrightarrow> Q' \<le> Q \<Longrightarrow> ht P' x Q' \<Longrightarrow> ht P (aprog P' x Q') Q"
+  by (hoarerule simp: aprog_def first: hl_classic)
 
 
 end
