Examples/Examples.thy
@@ -1,0 +1,367 @@
+theory Examples
+  imports "../Syntax"
+begin
+
+lemma hl_ret: "\<forall>s. ht P R {t. (z_update (\<lambda>_. y t) s) \<in> Q} \<Longrightarrow> ht P (block id R (\<lambda>s t. s) (\<lambda>s t. `z := y t)) Q"
+apply (rule hl_block)
+prefer 3
+apply (rule allI)+
+apply (rule hl_to_rel)
+apply (rule subset_refl)
+apply auto
+done
+
+lemma hl_no_changes: "\<forall>s m. Q \<subseteq> {t. (z_update (\<lambda>_. m) t) \<in> Q} \<Longrightarrow> ht Q (block id R (\<lambda>s t. s) (\<lambda>s t. `z := y t)) Q"
+by (force simp: block_def ht_def seq_def dyn_def to_rel_def)
+
+
+record state =
+    x :: nat
+    y :: nat
+    z :: nat
+    
+lemma swap:
+  "\<turnstile> \<lbrace>`x = xo \<and> `y = yo \<rbrace>
+      `z := `x;
+      `x := `y;
+      `y := `z
+   \<lbrace>`x = yo \<and> `y = xo\<rbrace>"
+   by hoare auto
+
+lemma "\<turnstile> \<lbrace> `x = n \<rbrace> 
+  local `x := `x + 1 in
+    `x := 2;
+    `y := `x + 1
+  end 
+  \<lbrace> `x = n \<and> `y = 3 \<rbrace>"
+  by hoare auto
+
+lemma "\<turnstile> \<lbrace> `x = u \<rbrace> local `x in R end \<lbrace> `x = u \<rbrace>"
+  apply (rule hl_block[where P'="\<lambda>s. {t. x s = u}" and R="\<lambda>s s'. {t. x t = u}"])
+  apply auto
+  by hoare
+
+definition proc :: "'s rel \<Rightarrow> ('s \<Rightarrow> 'v) \<Rightarrow> 's rel \<times> ('s \<Rightarrow> 'v)" where
+  "proc R v \<equiv> (R, v)"
+
+definition "MAX xo yo \<equiv> 
+      proc (`x := xo;
+      `y := yo;
+      \<lbrace> `x = xo \<and> `y = yo \<rbrace>
+      if `x \<ge> `y then
+        `y := `x
+      else
+        `y := `y
+      fi) y"
+
+lemma maximum: 
+  "\<turnstile> \<lbrace> `x = u \<and> `y = v \<rbrace> `z := call (MAX xo yo) \<lbrace> `z = max xo yo \<and> `x = u \<and> `y = v \<rbrace>"
+  unfolding MAX_def proc_def
+apply (rule hl_split)
+apply (rule hl_ret)
+apply simp
+apply hoare
+apply (rule hl_apre)
+apply hoare
+apply auto
+apply (rule hl_no_changes)
+apply force
+done
+
+lemma maximum: 
+  "\<turnstile> \<lbrace> `x = u \<rbrace> block id (MAX xo yo) (\<lambda>s t. s) (\<lambda>s t. `z := y t) \<lbrace> `x = u \<and> `z = max xo yo \<rbrace>"
+  unfolding MAX_def
+thm hl_ret
+apply (rule hl_split)
+defer
+apply (rule hl_ret)
+
+apply simp
+apply (rule allI)
+apply hoare
+apply (rule hl_apre)
+apply hoare
+apply auto
+apply (rule hl_no_changes)
+apply auto
+apply simp
+apply (rule hl_seq)
+apply (rule hl_seq)
+apply (rule hl_cond_tac)
+prefer 4
+apply (rule hl_to_rel)
+apply (rule subset_refl)
+prefer 3
+apply (rule hl_to_rel)
+apply (rule subset_refl)
+apply (rule subset_refl)
+apply clarify
+apply simp
+
+apply hoare
+apply auto
+
+
+
+lemma swap_annotated:
+  "\<turnstile> \<lbrace>`x = xo \<and> `y = yo \<rbrace>
+      `z := `x;
+      \<lbrace> `x = xo \<and> `y = yo \<and> `z = xo \<rbrace>
+      `x := `y;
+      \<lbrace> `x = yo \<and> `y = yo \<and> `z = xo \<rbrace>
+      `y := `z
+   \<lbrace>`x = yo \<and> `y = xo\<rbrace>"
+apply hoare
+apply auto
+done
+
+primrec fact :: "nat \<Rightarrow> nat" where
+  "fact 0 = 1"
+| "fact (Suc n) = (Suc n) * fact n"
+
+
+lemma fact: "\<turnstile> \<lbrace> True \<rbrace>
+  `x := 0;
+  `y := 1;
+  while `x \<noteq> xo
+  inv `y = fact `x
+  do
+    `x := `x + 1;
+    `y := `y * `x
+  od
+  \<lbrace> `y = fact xo \<rbrace>"
+  by hoare auto
+
+lemma fact_rec: "\<forall>xo. \<turnstile> \<lbrace> (xo = `x) \<rbrace>
+  rec Fact in
+    if `x = 0 then
+      `y := 1
+    else
+      `x := `x - 1;
+      \<lbrace> xo = `x + 1 \<rbrace>
+      Fact;
+      `x := `x + 1;
+      `y := `y \<cdot> `x
+    fi
+  end
+  \<lbrace> xo = `x \<rbrace>"
+apply (rule hl_rec2)
+prefer 2
+apply hoare
+apply force
+prefer 2
+apply (rule hl_apre)
+apply (rule subset_refl)
+apply simp
+apply (rule hl_apre3[where P="\<lambda>xo. {s. xo = Suc (x s)}"])
+apply assumption
+apply simp
+apply force
+
+sorry
+
+
+
+apply (erule_tac x="x sa - 1" in allE)
+apply hoare_step
+defer
+defer
+apply hoare_step
+apply hoare_step
+apply hoare_step
+apply hoare_step
+apply hoare_step
+apply hoare_step
+apply hoare_step
+apply hoare_step
+apply hoare_step
+apply simp
+prefer 3
+apply simp
+apply clarsimp
+apply assumption
+apply auto
+defer
+apply (rule hl_2[where P'="\<lambda>z u. {s. z = x s}" and Q'="\<lambda>z u. {s. z = x s}"])
+apply clarsimp
+apply clarsimp
+apply (rule allI)
+prefer 2
+apply clarsimp
+
+
+apply assumption
+apply clarsimp
+apply force
+
+
+apply hoare_step
+defer
+apply hoare_step
+prefer 3
+apply hoare_step
+apply hoare_step
+apply force
+prefer 2
+apply hoare_step
+apply hoare_step
+apply hoare_step
+apply hoare_step
+apply hoare_step
+apply hoare_step
+apply hoare_step
+apply simp_all
+apply (rule hl_conseq)
+apply hoare_step
+apply clarsimp
+prefer 2
+apply hoare_step
+apply hoare_step
+apply (rule conjI)
+apply (subgoal_tac "s \<in> {s. xo = Suc (x s)}")
+apply force
+apply assumption
+apply clarsimp
+apply (subst mem_Collect_eq)
+
+
+
+
+lemma "local `x := t in skip end = a" oops
+
+lemma [simp]: "ht P R <UNIV>"
+  apply (auto simp: ht_def seq_def)
+done
+
+lemma "P \<subseteq> UNIV" oops
+
+declare [[simp_trace]]
+lemma maximum2: 
+  "\<turnstile> \<lbrace> `x = xo \<rbrace> `x := 2; local `x in MAX end \<lbrace> `x = xo \<rbrace>"
+unfolding MAX_def
+apply hoare
+apply force
+apply safe
+apply force
+apply clarsimp
+apply auto
+
+apply (rule allI)
+apply (subst mem_Collect_eq)
+apply (rule subset_refl)
+
+apply simp
+apply auto
+apply (auto simp: ht_def seq_def)
+apply (rule subset_refl)
+
+apply (subst mem_Collect_eq)
+apply (rule allI)
+apply simp
+apply auto
+apply (unfold ht_def seq_def)
+apply simp
+apply auto
+apply (auto simp: ht_def)
+
+lemma maximum2: 
+  "\<turnstile> \<lbrace> `x = xo \<and> `y = yo\<rbrace> local `x := `x in (block id MAX (\<lambda>s t. s) (\<lambda>s t. \<langle>\<lambda>v. v \<lparr> z := y t \<rparr>\<rangle>)) end \<lbrace> `z = max xo yo \<and> `x = xo \<rbrace>"
+  unfolding MAX_def apply hoare
+  apply simp
+  apply (rule allI)
+  apply (subst Collect_mem_eq)
+apply (rule subset_refl)
+
+
+lemma euclids:
+  "\<turnstile> \<lbrace>`x = xo \<and> `y = yo\<rbrace> 
+    while `y \<noteq> 0
+    inv gcd `x `y = gcd xo yo
+    do 
+      `z := `y;
+      `y := `x mod `y;
+      `x := `z
+    od 
+    \<lbrace>gcd xo yo = `x\<rbrace>"
+  by (hoare, auto) (metis gcd_red_nat)
+
+record div_state = state +
+  q :: nat
+  r :: nat
+
+lemma div: 
+  "\<turnstile> \<lbrace> `x \<ge> 0 \<rbrace>
+    `q :=  0; `r := `x;
+    while `y \<le> `r
+    inv `x = `q * `y + `r \<and> `r \<ge> 0
+    do
+      `q := `q + 1;
+      `r := `r - `y
+    od
+  \<lbrace> `x = `q * `y + `r \<and> `r \<ge> 0 \<and> `r < `y \<rbrace>"
+  by hoare auto
+
+
+
+hide_const x y z q r
+
+lemma extend_euclid_invariant:
+  assumes "(a' :: int)\<cdot>m + b'\<cdot>n = c" "a\<cdot>m + b\<cdot>n = d" "c = q\<cdot>d + r"
+  shows "(a' - q\<cdot>a)\<cdot>m + (b'- q\<cdot>b)\<cdot>n = r"
+proof -
+  have "(a' - q\<cdot>a)\<cdot>m + (b'- q\<cdot>b)\<cdot>n = a'\<cdot>m - q\<cdot>a\<cdot>m + b'\<cdot>n - q\<cdot>b\<cdot>n"
+    by (metis add.left_commute int_distrib(3) uminus_add_conv_diff)
+  also have "... = a'\<cdot>m + b'\<cdot>n - q\<cdot>(a\<cdot>m + b\<cdot>n)"
+    proof -
+      have "\<And>u. u = d \<longrightarrow> u - b \<cdot> n = a \<cdot> m" by (simp add: assms(2) diff_eq_eq)
+      hence "c - d \<cdot> q + b \<cdot> (n \<cdot> q) = c - a \<cdot> (m \<cdot> q)" by (metis diff_add_eq diff_diff_eq2 int_distrib(3) mult.assoc mult.commute)
+      thus "a' \<cdot> m - q \<cdot> a \<cdot> m + b' \<cdot> n - q \<cdot> b \<cdot> n = a' \<cdot> m + b' \<cdot> n - q \<cdot> (a \<cdot> m + b \<cdot> n)" by (metis (no_types) assms(1) assms(2) diff_add_eq diff_eq_eq mult.commute mult.left_commute)
+    qed
+  finally show ?thesis
+    by (simp add: assms(1) assms(2) assms(3))
+qed
+
+
+record extended_euclid_state = 
+  a :: int
+  b :: int
+  a':: int
+  b':: int
+  c :: int
+  d :: int
+  r :: int
+  q :: int
+  t :: int
+
+(* Solve linear diophantine equations *)
+
+lemma extended_euclid: "\<turnstile> \<lbrace> True \<rbrace>
+    `b := 1;
+    `a':= 1;
+    `b' := 0;
+    `a := 0;
+    `c := m;
+    `d := n;
+    `q := `c div `d;
+    `r := `c mod `d;
+    while `r \<noteq> 0
+    inv
+      `a'\<cdot>m + `b'\<cdot>n = `c \<and> `a\<cdot>m + `b\<cdot>n = `d \<and> `c = `q\<cdot>`d + `r
+    do
+      `c := `d;
+      `d := `r;
+      `t := `a';
+      `a' := `a;
+      `a := `t - `q\<cdot>`a;
+      `t := `b';
+      `b' := `b;
+      `b := `t - `q\<cdot>`b;
+      `q := `c div `d;
+      `r := `c mod `d
+    od
+  \<lbrace> `a\<cdot>m + `b\<cdot>n = `d  \<rbrace>"
+  by (hoare, auto) (metis extend_euclid_invariant)
+
+hide_const a b a' b' c d r q t
+
+end
