ROOT
@@ -1,0 +1,10 @@
+session "Veritas" = "HOL" +
+  options [document = pdf, document_output = "output"]
+  theories [document = false]
+    (* Foo *)
+    (* Bar *)
+  theories
+    (* Baz *)
+    "Examples/Examples"
+  document_files
+    "root.tex"
